Add most of the parsing function
I still need to replace the length-ordering with lexicographic
ordering.

src/Parsers/NonComputational.v
@@ -1,5 +1,5 @@
 (** * Definition of a [comp]-based non-computational CFG parser *)
-Require Import Coq.Lists.List Coq.Program.Program Coq.Program.Wf.
+Require Import Coq.Lists.List Coq.Program.Program Coq.Program.Wf Coq.Arith.Wf_nat Coq.Arith.Compare_dec Coq.Classes.RelationClasses.
 Require Import Parsers.ContextFreeGrammar Parsers.Specification.
 Require Import Common ADTNotation.ilist.
 
@@ -26,12 +26,61 @@ Set Implicit Arguments.
 
 FIXME *)*)
 (** TODO: rename pattern to production *)
+
+Section wf.
+  Section wf_prod.
+    Context A B (RA : relation A) (RB : relation B).
+
+    Definition prod_relation : relation (A * B)
+      := fun ab a'b' =>
+           RA (fst ab) (fst a'b') \/ (fst a'b' = fst ab /\ RB (snd ab) (snd a'b')).
+
+    Fixpoint well_founded_prod_relation_helper
+             a b
+             (wf_A : Acc RA a) (wf_B : well_founded RB) {struct wf_A}
+    : Acc prod_relation (a, b)
+      := match wf_A with
+           | Acc_intro fa => (fix wf_B_rec b' (wf_B' : Acc RB b') : Acc prod_relation (a, b')
+                              := Acc_intro
+                                   _
+                                   (fun ab =>
+                                      match ab as ab return prod_relation ab (a, b') -> Acc prod_relation ab with
+                                        | (a'', b'') =>
+                                          fun pf =>
+                                            match pf with
+                                              | or_introl pf'
+                                                => @well_founded_prod_relation_helper
+                                                     _ _
+                                                     (fa _ pf')
+                                                     wf_B
+                                              | or_intror (conj pfa pfb)
+                                                => match wf_B' with
+                                                     | Acc_intro fb
+                                                       => eq_rect
+                                                            _
+                                                            (fun a'' => Acc prod_relation (a'', b''))
+                                                            (wf_B_rec _ (fb _ pfb))
+                                                            _
+                                                            pfa
+                                                   end
+                                            end
+                                      end)
+                             ) b (wf_B b)
+         end.
+
+    Definition well_founded_prod_relation : well_founded RA -> well_founded RB -> well_founded prod_relation.
+    Proof.
+      intros wf_A wf_B [a b]; hnf in *.
+      apply well_founded_prod_relation_helper; auto.
+    Defined.
+  End wf_prod.
+End wf.
+
 Local Open Scope string_like_scope.
 
 Section recursive_descent_parser.
   Context CharType (String : string_like CharType) (G : grammar CharType).
   Context (T : String -> nonterminal CharType -> Type)
-          (aggregate : forall s1 pat, T s1 [ [ pat ] ] -> forall s2 pats, T s2 [pats] -> T (s1 ++ s2)%string_like [pat::pats]%list)
           (T_reverse_lookup : forall str name, T str (Lookup G name) -> T str [ [ NonTerminal _ name ] ]).
   Context (parse_pattern_by_picking
            : forall (parse_pattern_from_split_list
@@ -42,34 +91,25 @@ Section recursive_descent_parser.
                     (pat : pattern CharType),
                T str [ pat ]).
   Context (decide_leaf : forall str ch, T str [ [ Terminal ch ] ]).
-  Context (make_empty : T (Empty _) [ [ ] ]).
   Context (fold_patterns : forall str (pats : list (pattern CharType)),
                              ilist (fun pat => T str [ pat ]) pats
                              -> T str pats).
+  (** FIXME: The type of the list of nonterminals should be able to
+  depend on the string we're parsing, so we can store proofs in it to
+  pass down the parse tree to handle impossible cases.  This will
+  require a [Total] lexicographic ordering on strings. *)
+  Context nonterminal_listT
+          (initial_nonterminal_data : nonterminal_listT)
+          (is_valid_nonterminal : nonterminal_listT -> nonterminal CharType -> bool)
+          (remove_nonterminal : nonterminal_listT -> nonterminal CharType -> nonterminal_listT)
+          (nonterminal_listT_R : nonterminal_listT -> nonterminal_listT -> Prop)
+          (remove_nonterminal_dec : forall ls nt, is_valid_nonterminal ls nt = true
+                                                  -> nonterminal_listT_R (remove_nonterminal ls nt) ls)
+          (ntl_wf : well_founded nonterminal_listT_R).
+  Context (make_abort : forall str nt valid_list, is_valid_nonterminal valid_list nt = false -> T str nt).
+
 
   Section parts.
-    Local Ltac t' :=
-      idtac;
-      match goal with
-        | _ => progress subst
-        | _ => exact id
-        | _ => assumption
-        | [ H : ?x <> ?x |- _ ] => solve [ destruct (H eq_refl) ]
-        | [ H : parse_of_item _ _ _ _ |- _ ] => inversion H; clear H
-        | [ H : parse_of_pattern _ _ _ _ |- _ ] => inversion H; clear H
-        | [ H : _ -> False |- False ] => apply H; clear H; solve [ repeat t' ]
-      end.
-
-    Class by_t' T := make_by_t' : T.
-    Hint Extern 0 (by_t' _) => unfold by_t'; solve [ repeat t' ] : typeclass_instances.
-
-    Local Ltac t :=
-      repeat match goal with
-               | [ |- False ] => clear abstract by_t' || fail 1
-               | _ => progress t'
-             end.
-
-
     Section item.
       Context (str : String)
               (parse_nonterminal : forall nt, T str nt).
@@ -107,14 +147,40 @@ Section recursive_descent_parser.
       End step.
 
       Section wf.
-        Check Fix.
-        SearchAbout well_founded.
-    End nonterminal
-                                        Proof.
-        refine (match nt with
-                  | nil => make_false str
-                  | pat::pats => _
-                end).
-      Definition parse_nonterminal str nt : T str nt
-        := reverse_nonterminal_permutation (parse_nonterminal_helper str (choose_nonterminal_order str nt)).
-    End nonterminal.
+        Definition parse_nonterminal_or_abort (valid_list : nonterminal_listT) (max_len : nat)
+                   (str : String)
+                   (pf : Length _ str <= max_len)
+                   (nt : nonterminal CharType)
+        : T str nt.
+        Proof.
+          revert str pf nt.
+          change max_len with (fst (max_len, valid_list)).
+          generalize (max_len, valid_list); clear max_len valid_list.
+          refine (@Fix (nat * nonterminal_listT) _ (well_founded_prod_relation
+                                                      lt_wf
+                                                      ntl_wf)
+                       _ _).
+          intros [max_len valid_list] parse_nonterminal str pf nt.
+          apply le_lt_eq_dec in pf; simpl in *.
+          destruct pf as [pf|pf].
+          { (** [str] got smaller, so we reset the valid nonterminals *)
+            destruct max_len as [|max_len]; [ solve [ destruct (Lt.lt_n_0 _ pf) ] | ].
+            exact (parse_nonterminal
+                     (max_len, initial_nonterminal_data)
+                     (or_introl (Lt.lt_n_Sn _))
+                     str
+                     (le_S_n _ _ pf)
+                     nt). }
+          { (** [str] didn't get smaller, so we cache the fact that we've hit this nonterminal already *)
+            case_eq (is_valid_nonterminal valid_list nt).
+            { (** It was valid, so we can remove it *)
+              intro H.
+              exact (parse_nonterminal
+                       (Length _ str, remove_nonterminal valid_list nt)
+                       (or_intror (conj (eq_sym pf) (remove_nonterminal_dec H)))
+                       str
+                       (reflexivity _)
+                       nt). }
+            { (** oops, we already saw this nonterminal in the past.  ABORT! *)
+              apply make_abort. } }
+        Defined.
